internal/examples/semantics/multiple_return.go
@@ -18,7 +18,7 @@ func returnThree() (uint64, bool, uint32) {
 	return 2, true, 1
 }
 
-func failing_testReturnThree() bool {
+func testReturnThree() bool {
 	x, y, z := returnThree()
 	return x == 2 && y == true && z == 1
 }
@@ -27,7 +27,7 @@ func returnFour() (uint64, bool, uint32, uint64) {
 	return 2, true, 1, 7
 }
 
-func failing_testReturnFour() bool {
+func testReturnFour() bool {
 	x, y, z, w := returnFour()
 	return x == 2 && y == true && z == 1 && w == 7
 }
